Formulate attacker strategies with winning distance nats

HML_Strategies_Game.thy
@@ -1,22 +1,39 @@
 theory HML_Strategies_Game
   imports
     Contrasim_Set_Game
-    HM_Logic_Infinitary
+    Contrasim_HML
 begin
 
-context c_set_game
+locale c_game_with_attacker_strategy  =
+  c_set_game trans \<tau>
+for
+  trans :: \<open>'s \<Rightarrow> 'a \<Rightarrow> 's \<Rightarrow> bool\<close> and
+  \<tau> :: \<open>'a\<close> +
+fixes
+  strat :: \<open>('s, 'a) c_set_game_node posstrategy\<close> and
+  winning_dist :: \<open>('s, 'a) c_set_game_node \<Rightarrow> nat\<close>
+assumes
+  winning_dist_decreasing: \<open>winning_dist (strat pos) < winning_dist pos\<close>
 begin
 
 text \<open>This construction of attacker formulas from a game only works if \<open>strat\<close> is a (non-cyclic)
   attacker strategy. (If it's winning and sound, the constructed formula should be distinguishing.)\<close>
 
-function attack_formula :: \<open>('s, 'a) c_set_game_node posstrategy \<Rightarrow> ('s, 'a) c_set_game_node \<Rightarrow> ('a,'s) HML_formula\<close> where
-  \<open>attack_formula strat (AttackerNode p Q) =
-    attack_formula strat (strat ((AttackerNode p Q)))\<close>
-| \<open>attack_formula strat (DefenderSimNode a p Q) =
-    (HML_poss a (attack_formula strat (AttackerNode p Q)))\<close>
-| \<open>attack_formula strat (DefenderSwapNode p Q) =
-    (HML_weaknor Q (\<lambda>q. (attack_formula strat (AttackerNode q {p}))))\<close>
+function attack_formula :: \<open>('s, 'a) c_set_game_node \<Rightarrow> ('a,'s) HML_formula\<close> where
+  \<open>attack_formula (AttackerNode p Q) =
+    attack_formula (strat ((AttackerNode p Q)))\<close>
+| \<open>attack_formula (DefenderSimNode a p Q) =
+    (HML_poss a (attack_formula (AttackerNode p Q)))\<close>
+| \<open>attack_formula (DefenderSwapNode p Q) =
+    (HML_weaknor Q (\<lambda>q. (attack_formula (AttackerNode q {p}))))\<close>
+  using c_set_game_defender_node.cases
+  by (auto, blast)
+
+termination attack_formula
+  using winning_dist_decreasing
+    wf_measure[of winning_dist]
+  unfolding wf_def
+  by auto
 
 end
 end
